Renamed query age to query date

Dafny/QueryBloodInventory.dfy
@@ -14,8 +14,8 @@ ensures result != null
 ensures result[..] == VerifyFilter(inv, inv.Length, (b: Blood) requires b != null reads b => b.GetBloodType() == bloodType)
 { result := Filter(inv, (b: Blood) requires b != null reads b => b.GetBloodType() == bloodType); }
 
-// Returns a new array containing only blood objects in a specified age range.
-method queryBloodByAge(inv: array<Blood>, start: int, end: int) returns (result: array<Blood>)
+// Returns a new array containing only blood objects in a specified date range.
+method queryBloodByDate(inv: array<Blood>, start: int, end: int) returns (result: array<Blood>)
 requires inv != null
 requires forall i | 0 <= i < inv.Length :: inv[i] != null
 ensures result != null
@@ -30,8 +30,8 @@ requires forall i | 0 <= i < inv.Length :: inv[i] != null
 reads set i | 0 <= i < inv.Length :: inv[i]
 { Matches(inv, inv.Length, (b: Blood) requires b != null reads b => b.GetBloodType() == bloodType) }
 
-// Returns the number of blood objects in a specified age range.
-function method countBloodByAge(inv: array<Blood>, start: int, end: int): int
+// Returns the number of blood objects in a specified date range.
+function method countBloodByDate(inv: array<Blood>, start: int, end: int): int
 reads inv
 requires inv != null
 requires forall i | 0 <= i < inv.Length :: inv[i] != null
